@prefix dcterms: <http://purl.org/dc/terms/> .
@prefix owl: <http://www.w3.org/2002/07/owl#> .
@prefix rdf: <http://www.w3.org/1999/02/22-rdf-syntax-ns#> .
@prefix rdfs: <http://www.w3.org/2000/01/rdf-schema#> .
@prefix vs: <http://www.w3.org/2003/06/sw-vocab-status/ns#> .
@prefix o: <http://omeka.org/s/vocabs/o#> .
@prefix cdash: <http://github.com/c-dash/ns/cdash/> .

## This file was originally created by the Custom Ontology module for Omeka.
## Subsequently it has been edited with a txt editor and imported using 
## the standard Omeka vocabulary import function. 

<http://github.com/c-dash/ns/cdash/> a owl:Ontology ;
    dcterms:title "CDASH Terms" ;
    dcterms:description "Terms for places and related resources" .

## Special properties to describe a Place.

# placeType has a custom picklist in CDASH  There are 7 basic place-types, including Building.
cdash:placeType a rdf:Property ;
    rdfs:label "Place Type" ;
    rdfs:comment "Choose from CDASH Place Types" ;
    rdfs:domain o:Resource ;
    vs:term_status "experimental" .

cdash:placeUse a rdf:Property ;
    rdfs:label "Place Use/s";
    rdfs:comment "Choose from http://www.getty.edu/research/tools/vocabularies/aat or consult CDASH documentation. 
    Example: Bank, Hardware Store";
    rdfs:domain o:Resource ;
    vs:term_status "experimental" .

cdash:bldgMaterial a rdf:Property ;
    rdfs:label "Building Material" ;
    rdfs:comment "Choose from http://www.getty.edu/research/tools/vocabularies/aat or consult CDASH documentation.
    Example: Brick, Reinforced Concrete";
    rdfs:domain o:Resource ;
    vs:term_status "experimental" .

cdash:mapLot a rdf:Property ;
    rdfs:label "Assessing Map-Lot" ;
    rdfs:comment "Look-Up at https://gis.cambridgema.gov/map ." ;
    rdfs:domain o:Resource ;
    vs:term_status "experimental" .

cdash:distDes a rdf:Property ;
    rdfs:label "District / Designation" ;
    rdfs:comment "Can be looked up at https://www.cambridgema.gov/historic/districtsHistoricProperties/districtsmap" ;
    rdfs:domain o:Resource ;
    vs:term_status "experimental" .

cdash:macrisID a rdf:Property ;
    rdfs:label "MACRIS Inventory Number" ;
    rdfs:comment "See http://mhc-macris.net
    Include a hyperlink to the MACRIS page for this place." ;
    rdfs:domain o:Resource ;
    vs:term_status "experimental" .

cdash:appearDate a rdf:Property ;
    rdfs:label "Appear Date" ;
    rdfs:comment "Date of earliest reference to the physical existence of this thing" ;
    rdfs:domain o:Resource ;
    vs:term_status "experimental" .

cdash:changeDate a rdf:Property ;
    rdfs:label "Date Renovated" ;
    rdfs:comment "Date associated with a change in this thing." ;
    rdfs:domain o:Resource ;
    vs:term_status "experimental" .

cdash:changeDesc a rdf:Property ;
    rdfs:label "Change Description" ;
    rdfs:comment "Describe a dated event in the life of this thing." ;
    rdfs:domain o:Resource ;
    vs:term_status "experimental" .

cdash:disappearDate a rdf:Property ;
    rdfs:label "Disappear Date" ;
    rdfs:comment "Earliest reference to the removal or demise of the thing." ;
    rdfs:domain o:Resource ;
    vs:term_status "experimental" .

cdash:dataQual a rdf:Property ;
    rdfs:label "Data Qualifiers" ;
    rdfs:comment "Notes about the sources and degree of confidence for properties quoted here." ;
    rdfs:domain o:Resource ;
    vs:term_status "experimental" .

cdash:streetAddress a rdf:Property ;
    rdfs:label "Street Address" ;
    rdfs:comment "Full street address.  Use house numbering and suffix guidelines from CDASH Documentation.
    Example: 77 Massachusetts Ave" ;
    rdfs:domain o:Resource ;
    vs:term_status "experimental" .

cdash:streetName a rdf:Property ;
    rdfs:label "Street Name" ;
    rdfs:comment "Include street name and suffix. Alternate spellings can be indicated by duplicating this property.  Use suffix abbreviations from CDASH Documentation.
    example: Massachusetts Ave" ;
    rdfs:domain o:Resource ;
    vs:term_status "experimental" .

cdash:houseNum a rdf:Property ;
    rdfs:label "House Number" ;
    rdfs:comment "The numeric part of the street address.
    example: '77'" ;
    rdfs:domain o:Resource ;
    vs:term_status "experimental" .

# Appears on both Place and Document items.
cdash:streetSort a rdf:Property ;
    rdfs:label "StreetSort Key" ;
    rdfs:comment "A string used to sort street addresses alphabetically.  The streetname comes first, then the number, left-padded with zeros to 6 characters.  In the case of items, append the document type.
    Example: 'Massachusetts-Ave_000077_Article or Monograph'" ;
    rdfs:domain o:Resource ;
    vs:term_status "experimental" .

cdash:locationScore a rdf:Property ;
    rdfs:label "Location Score" ;
    rdfs:comment "Estimate of location precision on a scale of 0 to 9" ;
    rdfs:domain o:Resource ;
    vs:term_status "experimental" .

## Properties particular to Building type places

cdash:bldgStyle a rdf:Property ;
    rdfs:label "Building Style/s" ;
    rdfs:comment "Choose from http://www.getty.edu/research/tools/vocabularies/aat or consult CDASH guidelines." ;
    rdfs:domain o:Resource ;
    vs:term_status "experimental" .

cdash:bldgMaterial a rdf:Property ;
    rdfs:label "Building Material/s" ;
    rdfs:comment "Choose from http://www.getty.edu/research/tools/vocabularies/aat or consult CDASH guidelines." ;
    rdfs:domain o:Resource ;
    vs:term_status "experimental" .

cdash:gisBldg a rdf:Property ;
    rdfs:label "GIS Building ID" ;
    rdfs:comment "Optional. Can be looked up at https://gis.cambridgema.gov/map ." ;
    rdfs:domain o:Resource ;
    vs:term_status "experimental" .

## personItem appears on Document or Place type items. It is a pointer to the identifier of a Place Item.
cdash:personItem a rdf:Property ;
    rdfs:label "CDASH Person" ;
    rdfs:comment "Select a CDASH Person associated with this resource." ;
    rdfs:domain o:Resource ;
    vs:term_status "experimental" .

## placeItem appears on Document or Person type items. It is a pointer to the identifier of a Place Item.
cdash:placeItem a rdf:Property ;
    rdfs:label "CDASH Place" ;
    rdfs:comment "Select a CDASH Place associated with this resource." ;
    rdfs:domain o:Resource ;
    vs:term_status "experimental" .